Prove compiled code only modifies cache variables
Any cache variable may be touched, but guarantees that user
abstractions are untouched. Add this postcondition to the generic spec
constructed for compiled code.

src/ConcurrentBridge.v
@@ -92,13 +92,11 @@ Module MakeBridge (C:CacheSubProtocol).
     exact (w, nil).
   Defined.
 
+  Definition cache_vars := [( vCache; vWriteBuffer; vDisk0; vdisk0; vdisk )].
+
   (* The idea of concurrent_spec is to compute a concurrent spec
      corresponding to sequential spec, capturing the same spec on top of
-     the abstraction exported by the cache.
-
-     TODO: need to also state only cache variables are modified, and thread
-     through all lemmas.
-   *)
+     the abstraction exported by the cache. *)
   Definition concurrent_spec R (spec: SeqHoareSpec R) : ConcurHoareSpec (Exc R) :=
     let 'SeqSpec pre post _ := spec in
     ConcurSpec
@@ -113,6 +111,7 @@ Module MakeBridge (C:CacheSubProtocol).
          | None => guar delta tid s s'
          end /\
          hashmap_le hm hm' /\
+         modified cache_vars s s' /\
          guar delta tid s_i' s').
 
   Ltac inv_exec' H :=
@@ -425,6 +424,37 @@ Module MakeBridge (C:CacheSubProtocol).
 
   Hint Resolve hashmap_le_upd.
 
+  Hint Immediate modified_refl.
+  Hint Resolve modified_reduce_strict.
+
+  Ltac prove_hincl :=
+    intros;
+    repeat match goal with
+    | [ H: HIn _ _ |- _ ] =>
+      inversion H; repeat sigT_eq; clear H
+    | [ |- HIn _ _ ] =>
+      solve [ repeat econstructor ]
+    end.
+
+  Lemma cache_disk0_cache_vars : forall t (v: var _ t),
+      HIn v [(vCache; vDisk0)] ->
+      HIn v cache_vars.
+  Proof.
+    prove_hincl.
+  Qed.
+
+  Hint Resolve cache_disk0_cache_vars.
+
+  Lemma cache_disk0_wb_disk_cache_vars :
+    forall (t : Type) (v0 : var (abstraction_types App.Sigma) t),
+      HIn v0 [(vCache; vDisk0; vWriteBuffer; vdisk)] ->
+      HIn v0 cache_vars.
+  Proof.
+    prove_hincl.
+  Qed.
+
+  Hint Resolve cache_disk0_wb_disk_cache_vars.
+
   Theorem cache_simulation_finish : forall T (p: Prog.prog T)
                                       (tid:TID) d hm m s_i s out,
       exec App.delta tid (compile p) (d, hm, m, s_i, s) out ->
@@ -433,10 +463,9 @@ Module MakeBridge (C:CacheSubProtocol).
           out = Finished (d', hm', m', s_i', s') (value v) ->
           (Prog.exec (project_disk s) hm p (Prog.Finished (project_disk s') hm' v) /\
            cacheI d' m' s' /\
-           (* here we shouldn't guarantee the full guar App.delta, only the
-           cache, since writes need not respect the global protocol *)
            guar delta tid s s' /\
            hashmap_le hm hm' /\
+           modified cache_vars s s' /\
            s_i' = s_i) \/
           (Prog.exec (project_disk s) hm p (Prog.Failed T))).
   Proof.
@@ -465,6 +494,7 @@ Module MakeBridge (C:CacheSubProtocol).
         unfold project_disk.
         simpl_match; auto.
         auto.
+        eauto.
       }
       {
         right.
@@ -493,6 +523,7 @@ Module MakeBridge (C:CacheSubProtocol).
         eapply PredCrash.possible_sync_respects_upd; eauto.
         apply possible_sync_refl.
         auto.
+        eauto.
       }
       {
         right.
@@ -540,6 +571,7 @@ Module MakeBridge (C:CacheSubProtocol).
         eapply Prog.XBindFinish; eauto.
         eapply cacheR_preorder; eauto.
         eapply hashmap_le_preorder; eauto.
+        eapply modified_trans; eauto.
       * left.
         split; intros; subst; exec_ret; inv_outcome.
   Qed.
@@ -565,6 +597,7 @@ Module MakeBridge (C:CacheSubProtocol).
       (cacheI d' m' s' /\
        guar delta tid s s' /\
        hashmap_le hm hm' /\
+       modified cache_vars s s' /\
        s_i' = s_i) \/
       (Prog.exec (project_disk s) hm p (Prog.Failed T)).
   Proof.
@@ -604,6 +637,7 @@ Module MakeBridge (C:CacheSubProtocol).
       intuition eauto.
       eapply cacheR_preorder; eauto.
       eapply hashmap_le_preorder; eauto.
+      eapply modified_trans; eauto.
       eapply Prog.XBindFinish; eauto.
       eapply Prog.XBindFail; eauto.
 
